GenAdd.v
@@ -1,0 +1,515 @@
+
+Require Import Arith Lia Wf_nat List Bool.
+Require Import DeltaList FunG GenFib GenG.
+Import ListNotations.
+Set Implicit Arguments.
+
+(** Study of quasi-additivity for [f k n] function defined in [GenG]:
+    [f k (p+n)] is close to [f k p + f k n].
+    Said otherwise, for some fixed p, few values are reached by
+    [f k (p+n)-f k n] when n varies.
+    For this study, we'll turn a strict k-decomposition of n into
+    a lax decomp of (p+n).
+*)
+
+Lemma rev_inj {A} (l l' : list A) : rev l = rev l' -> l = l'.
+Proof.
+ intros. now rewrite <- (rev_involutive l), H, rev_involutive.
+Qed.
+
+Lemma rev_switch {A} (l l' : list A) : rev l = l' -> l = rev l'.
+Proof.
+ intros. now rewrite <- (rev_involutive l), H.
+Qed.
+
+(** Cut a decomposition in two, all the left being < p *)
+
+Fixpoint cut_lt_ge p l :=
+ match l with
+ | [] => ([],[])
+ | a::l' => if p <=? a then ([],l)
+            else let '(l1,l2) := cut_lt_ge p l' in (a::l1,l2)
+ end.
+
+Lemma cut_app p l :
+  let '(l1,l2) := cut_lt_ge p l in l1++l2 = l.
+Proof.
+ induction l; simpl; auto.
+ case Nat.leb_spec; simpl; auto. intros LE.
+ destruct cut_lt_ge. simpl. f_equal. auto.
+Qed.
+
+Lemma cut_fst p l :
+  Below (fst (cut_lt_ge p l)) p.
+Proof.
+ induction l as [|a l IH]; simpl.
+ - unfold Below; simpl. intuition.
+ - case Nat.leb_spec.
+   + unfold Below; simpl; intuition.
+   + destruct cut_lt_ge. unfold Below in *; simpl in *. intuition.
+Qed.
+
+Lemma cut_snd p l a l':
+  snd (cut_lt_ge p l) = a::l' -> p <= a.
+Proof.
+ induction l as [|b l IH]; simpl.
+ - inversion 1.
+ - case Nat.leb_spec.
+   + simpl. intros LT [= -> ->]; auto.
+   + intros _. destruct cut_lt_ge. simpl in *; auto.
+Qed.
+
+Lemma cut_snd' k p l :
+  Delta k l ->
+  forall x, In x (snd (cut_lt_ge p l)) -> p <= x.
+Proof.
+ generalize (cut_app p l) (cut_snd p l).
+ destruct (cut_lt_ge p l) as (l1,l2). simpl.
+ intros <-. rewrite Delta_app_iff. intros H (_ & H' & _).
+ destruct l2 as [|a l2]; simpl.
+ - inversion 1.
+ - specialize (H a l2 eq_refl).
+   intros x [<-|IN]; auto.
+   transitivity a; auto. eapply Delta_le; eauto.
+Qed.
+
+(* To add p to a strict k-decomposition (while possibly relaxing it),
+   no need to dig deeper than value [invA_up k p + 3*k-1].
+   Note : tighter upper bounds than that could probably be found,
+   but seem harder to prove *)
+
+Definition bound_idx k p := invA_up k p + 3*k-1.
+
+Definition low_high k p l := cut_lt_ge (bound_idx k p) l.
+
+Definition addlow k p low :=
+ match rev low with
+ | [] => decomp k p
+ | a::rlow' =>
+   let u:=invA_up k p +k-1 in
+   if u <? a then
+     (* a is big enough : putting (S a) instead of a in the decomposition
+        adds at least p (while remaining lax). *)
+     decompminus k (rev rlow'++[S a]) (A k (a-k) - p)
+   else
+     (* a is low enough : we can add an extra term in the decomposition *)
+     decompminus k (low ++[u+k]) (A k (u+k) - p)
+ end.
+
+Lemma addlow_sum k p l : k<>0 ->
+  let low := fst (low_high k p l) in
+  sumA k (addlow k p low) = p + sumA k low.
+Proof.
+ intros Hk.
+ destruct (low_high k p l) as (low,high) eqn:E. simpl.
+ unfold addlow.
+ destruct (rev low) as [|a rlow'] eqn:E'.
+ - apply rev_switch in E'. rewrite decomp_sum, E'. simpl; auto.
+ - apply rev_switch in E'. simpl in E'.
+   set (u := invA_up k p + k - 1).
+   case Nat.ltb_spec; intros.
+   + rewrite decompminus_sum, E'.
+     rewrite !sumA_app.
+     cbn - [A]. rewrite A_S.
+     assert (p <= A k (a-k)); try lia.
+     { etransitivity. apply (invA_up_spec k). apply A_mono. lia. }
+   + rewrite decompminus_sum. rewrite sumA_app. simpl.
+     assert (p <= A k (u+k)); try lia.
+     { etransitivity. apply (invA_up_spec k). apply A_mono. lia. }
+Qed.
+
+Definition addlow_delta k p l : k<>0 -> Delta (S k) l ->
+  let (low,high) := low_high k p l in
+  Delta k (addlow k p low ++ high).
+Proof.
+ intros Hk D.
+ set (u := bound_idx k p).
+ generalize (cut_app u l) (cut_fst u l) (cut_snd' u D).
+ change (cut_lt_ge _ _) with (low_high k p l).
+ destruct (low_high k p l) as (low,high). simpl.
+ intros E Hlow Hhigh.
+ unfold addlow.
+ destruct (rev low) as [|a rlow'] eqn:E'.
+ - apply rev_switch in E'. subst low. simpl in E. subst high.
+   apply Delta_app_iff. repeat split; auto using decomp_delta.
+   intros x x' IN IN'. apply Hhigh in IN'.
+   transitivity u; auto with arith.
+   assert (A k x <= p).
+   { rewrite <- (decomp_sum k p). apply sumA_in_le; auto. }
+   assert (x <= invA_up k p).
+   { apply (@A_le_inv k).
+     transitivity p; auto. apply invA_up_spec. }
+   unfold bound_idx in u. lia.
+ - apply rev_switch in E'. simpl in E'.
+   set (v := invA_up k p + k-1).
+   subst l.
+   rewrite Delta_app_iff in D. destruct D as (D1 & D2 & D3).
+   case Nat.ltb_spec; intros.
+   + apply decompminus_app_delta.
+     rewrite Delta_app_iff. repeat split; auto.
+     eapply Delta_up_last with a; auto. rewrite <- E'; auto.
+     intros x x' IN IN'.
+     rewrite in_app_iff in IN. destruct IN as [IN|[<-|[ ]]].
+     * specialize (D3 x x').
+       rewrite E', in_app_iff in D3.
+       specialize (D3 (or_introl IN) IN'). lia.
+     * specialize (D3 a x').
+       rewrite E', in_app_iff in D3.
+       specialize (D3 (or_intror (or_introl eq_refl)) IN'). lia.
+   + apply decompminus_app_delta.
+     rewrite <- app_assoc. apply Delta_app_iff; repeat split; auto.
+     * rewrite Delta_app_iff; repeat split; auto.
+       intros x x' [<-|[ ]] IN'. specialize (Hhigh x' IN').
+       unfold bound_idx in u. lia.
+     * intros x x'. rewrite in_app_iff.
+       intros IN [[<-|[ ]]|IN'].
+       { rewrite E' in *. assert (LE := Delta_last_le _ _ _ D1 IN). lia. }
+       { specialize (D3 x x' IN IN'). lia. }
+Qed.
+
+(* So, all values taken by [f k (p+n)-f k n] when n varies in [nat] are
+   values that are already encountered when n varies in just
+   [0..add_bound k p[. *)
+
+Definition add_bound k p := A k (bound_idx k p).
+
+Definition reduced k p n := sumA k (fst (low_high k p (decomp k n))).
+
+Lemma reduced_lt k p n :
+  reduced k p n < add_bound k p.
+Proof.
+ unfold reduced, add_bound.
+ assert (D := decomp_delta k n).
+ set (l := decomp k n) in *. clearbody l.
+ assert (E := cut_app (bound_idx k p) l).
+ assert (B := cut_fst (bound_idx k p) l).
+ change (cut_lt_ge _ _) with (low_high k p l) in E,B.
+ destruct (low_high k p l) as (low,high) eqn:E'. simpl in *.
+ rewrite <-E in D.
+ rewrite Delta_app_iff in D. destruct D as (D1 & D2 & D3).
+ destruct (rev low) as [|a rlow'] eqn:E''.
+ - apply rev_switch in E''. subst low. simpl.
+   generalize (@A_nz k (bound_idx k p)). lia.
+ - rewrite <- sumA_rev, E''.
+   apply Nat.lt_le_trans with (A k (S a)).
+   + apply decomp_max. rewrite <- E''. now apply DeltaRev_rev.
+   + apply A_mono. specialize (B a).
+     rewrite in_rev, E'' in B. simpl in B. intuition.
+Qed.
+
+Lemma additivity_reduced k p : k<>0 ->
+ forall n,
+   let m := reduced k p n in
+   f k (p+n) - f k n = f k (p+m) - f k m.
+Proof.
+ intros Hk n.
+ assert (D := decomp_delta k n).
+ unfold reduced; simpl.
+ rewrite <- (decomp_sum k n) at 1 2.
+ set (l := decomp k n) in *. clearbody l.
+ assert (E := cut_app (bound_idx k p) l).
+ change (cut_lt_ge _ _) with (low_high k p l) in E.
+ assert (E' := @addlow_sum k p l Hk).
+ assert (D' := @addlow_delta k p l Hk D).
+ destruct (low_high k p l) as (low,high). simpl in *.
+ subst l.
+ rewrite sumA_app at 1.
+ rewrite Nat.add_assoc, <- E', <- !sumA_app.
+ rewrite !f_sumA_lax; auto.
+ - rewrite !map_app, !sumA_app. lia.
+ - rewrite Delta_app_iff in D. intuition.
+ - rewrite Delta_app_iff in D'. intuition.
+Qed.
+
+Lemma additivity_bounded k p : k<>0 ->
+ forall n, exists m,
+   m < add_bound k p /\
+   f k (p+n) - f k n = f k (p+m) - f k m.
+Proof.
+ intros Hk n. exists (reduced k p n). split.
+ - apply reduced_lt.
+ - now apply additivity_reduced.
+Qed.
+
+(** We could hence prove bounds for [f k (p+n)-f k p] by computation. *)
+
+Fixpoint map2 {A B C}(f:A->B->C) l1 l2 :=
+  match l1,l2 with
+  | x1::l1', x2::l2' => f x1 x2 :: map2 f l1' l2'
+  | _, _ => []
+  end.
+
+Definition all_diffs k p :=
+  let stk := ftabulate k (p + (add_bound k p - 1)) in
+  map2 Nat.sub stk (npop p stk).
+
+Lemma all_diffs_spec k p :
+  all_diffs k p =
+  map (fun x => f k (p+x)-f k x) (countdown (add_bound k p - 1)).
+Proof.
+ unfold all_diffs.
+ set (m := add_bound _ _ - 1). clearbody m.
+ rewrite ftabulate_spec.
+ rewrite npop_map.
+ replace p with ((p+m)-m) at 2 by lia.
+ rewrite npop_countdown by lia.
+ induction m.
+ - simpl. destruct p; simpl; auto. f_equal. now destruct countdown.
+ - rewrite Nat.add_succ_r. simpl. f_equal; auto.
+Qed.
+
+Definition check_additivity test k p :=
+  forallb test (all_diffs k p).
+
+Lemma check_additivity_spec test k p : k<>0 ->
+  check_additivity test k p = true ->
+  forall n, test (f k (p+n)-f k n) = true.
+Proof.
+ intros Hk E. unfold check_additivity in E.
+ rewrite forallb_forall in E.
+ intros n. destruct (@additivity_bounded k p Hk n) as (m & Hm & ->).
+ apply E. rewrite all_diffs_spec.
+ rewrite in_map_iff. exists m. split; auto.
+ rewrite countdown_in. lia.
+Qed.
+
+Lemma decide_additivity k p a b : k<>0 ->
+ check_additivity (fun m => andb (a <=? m) (m <=? b)) k p = true ->
+ forall n, a + f k n <= f k (p+n) <= b + f k n.
+Proof.
+ intros.
+ assert (f k n <= f k (p+n)) by (apply f_mono; lia).
+ assert (a <= f k (p+n) - f k n <= b); try lia.
+ { rewrite <- !Nat.leb_le.
+   rewrite <- andb_true_iff.
+   change ((fun m => andb (a <=? m) (m <=? b)) (f k (p+n)-f k n) = true).
+   clear H1. revert n.
+   apply check_additivity_spec; auto. }
+Qed.
+
+
+(** Particular case of function H, i.e. k=2 *)
+
+Definition h := f 2.
+
+Lemma h_add_1 n : h n <= h (1+n) <= 1 + h n.
+Proof.
+ unfold h. destruct (f_step 2 n); simpl; lia.
+Qed.
+
+Lemma h_add_2 n : 1 + h n <= h (2+n) <= 2 + h n.
+Proof.
+ apply decide_additivity. auto. now vm_compute.
+Qed.
+
+Lemma h_add_3 n : 1 + h n <= h (3+n) <= 3 + h n.
+Proof.
+ apply decide_additivity. auto. now vm_compute.
+Qed.
+
+Lemma h_add_4 n : 2 + h n <= h (4+n) <= 3 + h n.
+Proof.
+ apply decide_additivity. auto. now vm_compute.
+Qed.
+
+Lemma h_add_5 n : 3 + h n <= h (5+n) <= 4 + h n.
+Proof.
+ apply decide_additivity. auto. now vm_compute.
+Qed.
+
+Lemma h_add_6 n : 3 + h n <= h (6+n) <= 5 + h n.
+Proof.
+ apply decide_additivity. auto. now vm_compute.
+Qed.
+
+Lemma h_add_7 n : 4 + h n <= h (7+n) <= 6 + h n.
+Proof.
+ apply decide_additivity. auto. now vm_compute.
+Qed.
+
+Lemma h_add_8 n : 5 + h n <= h (8+n) <= 6 + h n.
+Proof.
+ apply decide_additivity. auto. now vm_compute.
+Qed.
+
+Lemma h_add_9 n : 5 + h n <= h (9+n) <= 7 + h n.
+Proof.
+ apply decide_additivity. auto. now vm_compute.
+Qed.
+
+Lemma h_add_10 n : 6 + h n <= h (10+n) <= 8 + h n.
+Proof.
+ apply decide_additivity. auto. now vm_compute.
+Qed.
+
+(* h(18+n) = h n + h 18 + [-2..0] *)
+Lemma h_add_18 n : 11 + h n <= h (18+n) <= 13 + h n.
+Proof.
+ apply decide_additivity. auto. now vm_compute.
+Qed.
+
+(* For comparison with f 3 *)
+Lemma h_add_33 n : 22 + h n <= h (33+n) <= 23 + h n.
+Proof.
+ apply decide_additivity. auto. now vm_compute.
+Qed.
+
+(* h(39+n) = h n + h 39 + [0..2] *)
+Lemma h_add_39 n : 26 + h n <= h (39+n) <= 28 + h n.
+Proof.
+ apply decide_additivity. auto. now vm_compute.
+Qed.
+
+(* TODO: experimentally, h(n+m)-h(n)-h(m) is in [-2..2] in general
+         and in [-1..1] when m is a [A 2] number.
+   Proof: ??
+*)
+
+(* Combined with g_add_8, h_add_8 is enough to show that g <= h *)
+
+Lemma g_below_h n : g n <= h n.
+Proof.
+induction n as [n IH] using lt_wf_ind.
+destruct (Nat.lt_ge_cases n 8).
+- do 8 (destruct n; [compute; auto|]). lia.
+- replace n with (8+(n-8)) by lia.
+  transitivity (5 + g (n - 8)). apply g_add_8.
+  transitivity (5 + h (n - 8)). 2:apply h_add_8.
+  specialize (IH (n-8)). lia.
+Qed.
+
+(* TODO: g_below_h can be generalized into :
+   Conjecture : forall k n, f k n <= f (S k) n
+   Proof : ??
+*)
+
+(* f 3 *)
+
+Lemma fk_add_1 k n : f k n <= f k (1+n) <= 1 + f k n.
+Proof.
+ unfold h. destruct (f_step k n); simpl; lia.
+Qed.
+
+Lemma fk_add_2 k n : 1 + f k n <= f k (2+n) <= 2 + f k n.
+Proof.
+ unfold h. split.
+ - generalize (f_SS k n). simpl. lia.
+ - apply f_le_add.
+Qed.
+
+Lemma fk_add_3 k n : 1 + f k n <= f k (3+n) <= 3 + f k n.
+Proof.
+ split.
+ - transitivity (f k (2+n)). apply fk_add_2. apply f_mono. lia.
+ - apply f_le_add.
+Qed.
+
+Lemma fk_add_4 k n : 2 + f k n <= f k (4+n) <= 4 + f k n.
+Proof.
+ split.
+ - transitivity (1 + f k (2 + n)).
+   + generalize (fk_add_2 k n). lia.
+   + apply (fk_add_2 k (2+n)).
+ - apply f_le_add.
+Qed.
+
+Lemma f3_add_5 n : 3 + f 3 n <= f 3 (5+n) <= 4 + f 3 n.
+Proof.
+ apply decide_additivity. auto. now vm_compute.
+Qed.
+
+Lemma f3_add_6 n : 3 + f 3 n <= f 3 (6+n) <= 5 + f 3 n.
+Proof.
+ apply decide_additivity. auto. now vm_compute.
+Qed.
+
+Lemma f3_add_7 n : 4 + f 3 n <= f 3 (7+n) <= 6 + f 3 n.
+Proof.
+ apply decide_additivity. auto. now vm_compute.
+Qed.
+
+Lemma f3_add_8 n : 5 + f 3 n <= f 3 (8+n) <= 7 + f 3 n.
+Proof.
+ apply decide_additivity. auto. now vm_compute.
+Qed.
+
+Lemma f3_add_9 n : 6 + f 3 n <= f 3 (9+n) <= 8 + f 3 n.
+Proof.
+ apply decide_additivity. auto. now vm_compute.
+Qed.
+
+Lemma f3_add_10 n : 6 + f 3 n <= f 3 (10+n) <= 8 + f 3 n.
+Proof.
+ apply decide_additivity. auto. now vm_compute.
+Qed.
+
+Lemma f3_add_33 n : 23 + f 3 n <= f 3 (33+n) <= 25 + f 3 n.
+Proof.
+ apply decide_additivity. auto. now vm_compute.
+Qed.
+
+(* TODO general bounds for f3(n+m)-f3(n)-f3(m) ??
+   Same for any fk ??
+*)
+
+Lemma h_below_f3 n : h n <= f 3 n.
+Proof.
+induction n as [n IH] using lt_wf_ind.
+destruct (Nat.lt_ge_cases n 33).
+- clear IH.
+  unfold h. rewrite <- !fopt_spec.
+  do 33 (destruct n; [vm_compute; auto|]). exfalso. lia.
+- replace n with (33+(n-33)) by lia.
+  transitivity (23 + h (n - 33)). apply h_add_33.
+  transitivity (23 + f 3 (n - 33)).
+  specialize (IH (n-33)). lia.
+  apply (f3_add_33 (n-33)).
+Qed.
+
+Lemma f3_add_73 n : 51 + f 3 n <= f 3 (73+n) <= 54 + f 3 n.
+Proof.
+ apply decide_additivity. auto. now vm_compute.
+Qed.
+
+Lemma f4_add_73 n : 54 + f 4 n <= f 4 (73+n) <= 57 + f 4 n.
+Proof.
+ apply decide_additivity. auto. now vm_compute.
+Qed.
+
+Lemma f3_below_f4 n : f 3 n <= f 4 n.
+Proof.
+induction n as [n IH] using lt_wf_ind.
+destruct (Nat.lt_ge_cases n 73).
+- clear IH.
+  rewrite <- !fopt_spec.
+  do 73 (destruct n; [vm_compute; auto|]). exfalso. lia.
+- replace n with (73+(n-73)) by lia.
+  transitivity (54 + f 3 (n - 73)). apply (f3_add_73 (n-73)).
+  transitivity (54 + f 4 (n - 73)).
+  specialize (IH (n-73)). lia.
+  apply (f4_add_73 (n-73)).
+Qed.
+
+Lemma f4_add_169 n : 125 + f 4 n <= f 4 (169+n) <= 129 + f 4 n.
+Proof.
+ apply decide_additivity. auto. now vm_compute.
+Qed.
+
+Lemma f5_add_169 n : 129 + f 5 n <= f 5 (169+n) <= 135 + f 5 n.
+Proof.
+ apply decide_additivity. auto. now vm_compute.
+Qed.
+
+Lemma f4_below_f5 n : f 4 n <= f 5 n.
+Proof.
+induction n as [n IH] using lt_wf_ind.
+destruct (Nat.lt_ge_cases n 169).
+- clear IH.
+  rewrite <- !fopt_spec.
+  do 169 (destruct n; [vm_compute; auto|]). exfalso. lia.
+- replace n with (169+(n-169)) by lia.
+  transitivity (129 + f 4 (n - 169)). apply (f4_add_169 (n-169)).
+  transitivity (129 + f 5 (n - 169)).
+  specialize (IH (n-169)). lia.
+  apply (f5_add_169 (n-169)).
+Qed.
